***NO_CI*** Commented out the lemmas used to push through MRef.fst as it should go through without them.

ulib/FStar.Heap.fst
@@ -9,7 +9,7 @@ open FStar.Monotonic.Heap
    reference to be allocated) and a mapping of allocated raw 
    references (represented as natural numbers) to types and values. *)
 
-let heap = heap
+abstract let heap = heap
 
 abstract let ref (a:Type0) = mref a (fun _ _ -> True)
 
@@ -25,31 +25,25 @@ abstract let compare_addrs (#a:Type) (#b:Type) (r1:ref a) (r2:ref b)
 
 abstract let contains (#a:Type0) (h:heap) (r:ref a) = contains h (as_mref r) 
 
-abstract let unused_in (#a:Type) (r:ref a) (h:heap) :Type0 = unused_in r h
+abstract let unused_in (#a:Type) (r:ref a) (h:heap) :Type0 = unused_in (as_mref r) h
 
 let fresh (#a:Type) (r:ref a) (h0:heap) (h1:heap) = fresh (as_mref r) h0 h1
-
-let lemma_fresh_not_contained (#a:Type) (r:ref a) (h0:heap) (h1:heap) 
-  :Lemma (requires (fresh r h0 h1))
-         (ensures  (~(contains h0 r)))
-	 [SMTPat (fresh r h0 h1)]
-  = lemma_fresh_not_contained r h0 h1
 
 let only x = singleton (addr_of x)
 
 (* Select. *)
 private abstract let sel_tot (#a:Type) (h:heap) (r:ref a{h `contains` r}) :a
-  = sel_tot h r
+  = sel_tot h (as_mref r)
 
 abstract let sel (#a:Type) (h:heap) (r:ref a) :GTot a
-  = sel h r
+  = sel h (as_mref r)
 
 (* Update. *)
 abstract let upd_tot (#a:Type) (h:heap) (r:ref a{h `contains` r}) (x:a) :heap
-  = upd_tot h r x
+  = upd_tot h (as_mref r) x
 
 abstract let upd (#a:Type) (h:heap) (r:ref a) (x:a) :GTot heap
-  = upd h r x
+  = upd h (as_mref r) x
 
 (* Allocate. *)
 abstract let alloc (#a:Type) (h:heap) (x:a) (mm:bool) :GTot (ref a * heap)
@@ -57,11 +51,81 @@ abstract let alloc (#a:Type) (h:heap) (x:a) (mm:bool) :GTot (ref a * heap)
   
 abstract let free_mm (#a:Type) (h:heap) (r:ref a{h `contains` r /\ is_mm r})
   :GTot heap
-  = free_mm h r
+  = free_mm h (as_mref r)
 
 let modifies (s:set nat) (h0:heap) (h1:heap) = modifies s h0 h1
 
 (** some lemmas that summarize the behavior **)
+
+
+(*
+ * update of a well-typed reference
+ *)
+private let lemma_upd_contains_test
+  (#a:Type) (h0:heap) (r:ref a) (x:a)
+  :Lemma (h0 `contains` r ==>
+          (let h1 = upd h0 r x in
+           (forall (b:Type) (r':ref b). addr_of r' <> addr_of r ==> sel h0 r' == sel h1 r') /\
+	   (forall (b:Type) (r':ref b). h0 `contains` r' <==> h1 `contains` r')             /\
+	   (forall (b:Type) (r':ref b). r' `unused_in` h0  <==> r' `unused_in` h1)))
+  = ()
+
+(*
+ * update of a reference that is mapped but not necessarily well-typed
+ * we cannot prove that h0 `contains` r' ==> h1 `contains` r'
+ * because consider that in h0 (r:ref a) contains (| b, y:b |),
+ * and that (r':ref b) s.t. r'.addr = r.addr
+ * in h0, r' is well-typed, but in h1 it's not
+ *)
+private let lemma_upd_contains_not_necessarily_well_typed_test
+  (#a:Type) (h0:heap) (r:ref a) (x:a)
+  :Lemma ((~ (r `unused_in` h0)) ==>
+          (let h1 = upd h0 r x in
+	   h1 `contains` r /\
+           (forall (b:Type) (r':ref b). addr_of r' <> addr_of r ==> sel h0 r' == sel h1 r')           /\
+	   (forall (b:Type) (r':ref b). (addr_of r' <> addr_of r /\ h0 `contains` r') ==> h1 `contains` r') /\
+	   (forall (b:Type) (r':ref b). r' `unused_in` h0 <==> r' `unused_in` h1)))
+  = ()
+
+(*
+ * update of an unused reference
+ *)
+private let lemma_upd_unused_test
+  (#a:Type) (h0:heap) (r:ref a) (x:a)
+  :Lemma (r `unused_in` h0 ==>
+          (let h1 = upd h0 r x in
+	   h1 `contains` r /\
+           (forall (b:Type) (r':ref b). addr_of r' <> addr_of r ==> sel h0 r' == sel h1 r') /\
+	   (forall (b:Type) (r':ref b). h0 `contains` r' ==> h1 `contains` r')             /\
+	   (forall (b:Type) (r':ref b). ~ (r' `unused_in` h0) ==> ~ (r' `unused_in` h1))))
+  = ()
+
+(*
+ * alloc and alloc_mm behaves just like upd of an unmapped reference
+ *)
+private let lemma_alloc_test (#a:Type) (h0:heap) (x:a) (mm:bool)
+  :Lemma (let (r, h1) = alloc h0 x mm in
+          r `unused_in` h0 /\
+	  h1 `contains` r  /\
+          is_mm r = mm     /\
+          (forall (b:Type) (r':ref b). addr_of r' <> addr_of r ==> sel h0 r' == sel h1 r') /\
+          (forall (b:Type) (r':ref b). h0 `contains` r' ==> h1 `contains` r')             /\
+	  (forall (b:Type) (r':ref b). ~ (r' `unused_in` h0) ==> ~ (r' `unused_in` h1)))
+  = ()
+
+private let lemma_free_mm_test (#a:Type) (h0:heap) (r:ref a{h0 `contains` r /\ is_mm r})
+  :Lemma (let h1 = free_mm h0 r in
+          r `unused_in` h1 /\
+	  (forall (b:Type) (r':ref b). addr_of r' <> addr_of r ==>
+	                          ((sel h0 r' == sel h1 r'                 /\
+				   (h0 `contains` r' <==> h1 `contains` r') /\
+				   (r' `unused_in` h0 <==> r' `unused_in` h1)))))
+  = ()
+
+private let lemma_alloc_fresh_test (#a:Type) (h0:heap) (x:a) (mm:bool)
+  :Lemma (let r, h1 = alloc h0 x mm in
+          fresh r h0 h1 /\ modifies empty h0 h1)
+  = ()
 
 (** **)
 
@@ -70,21 +134,21 @@ let lemma_contains_implies_used
   :Lemma (requires (h `contains` r))
          (ensures  (~ (r `unused_in` h)))
 	 [SMTPatOr [[SMTPat (h `contains` r)]; [SMTPat (r `unused_in` h)]]]
-  = lemma_contains_implies_used h r
+  = lemma_contains_implies_used h (as_mref r)
 
 let lemma_distinct_addrs_distinct_types
   (#a:Type) (#b:Type) (h:heap) (r1:ref a) (r2:ref b)
   :Lemma (requires (a =!= b /\ h `contains` r1 /\ h `contains` r2))
          (ensures  (addr_of r1 <> addr_of r2))
 	 [SMTPatT (h `contains` r1); SMTPatT (h `contains` r2)]
-  = lemma_distinct_addrs_distinct_types h r1 r2
+  = lemma_distinct_addrs_distinct_types h (as_mref r1) (as_mref r2)
 
 let lemma_distinct_addrs_unused
   (#a:Type) (#b:Type) (h:heap) (r1:ref a) (r2:ref b)
   :Lemma (requires (r1 `unused_in` h /\ ~ (r2 `unused_in` h)))
          (ensures  (addr_of r1 <> addr_of r2))
          [SMTPat (r1 `unused_in` h); SMTPat (r2 `unused_in` h)]
-  = lemma_distinct_addrs_unused h r1 r2
+  = lemma_distinct_addrs_unused h (as_mref r1) (as_mref r2)
 
 let lemma_alloc (#a:Type) (h0:heap) (x:a) (mm:bool)
   :Lemma (requires True)
@@ -97,14 +161,14 @@ let lemma_free_mm_sel (#a:Type) (#b:Type) (h0:heap) (r:ref a{h0 `contains` r /\ 
   :Lemma (requires True)
          (ensures  (addr_of r' <> addr_of r ==> sel h0 r' == sel (free_mm h0 r) r'))
 	 [SMTPat (sel (free_mm h0 r) r')]
-  = lemma_free_mm_sel h0 r r'
+  = lemma_free_mm_sel h0 (as_mref r) (as_mref r')
 
 let lemma_free_mm_contains (#a:Type) (#b:Type) (h0:heap) (r:ref a{h0 `contains` r /\ is_mm r}) (r':ref b)
   :Lemma (requires True)
          (ensures  (let h1 = free_mm h0 r in
 	            (addr_of r' <> addr_of r /\ h0 `contains` r') <==> h1 `contains` r'))
 	 [SMTPat ((free_mm h0 r) `contains` r')]
-  = lemma_free_mm_contains h0 r r'
+  = lemma_free_mm_contains h0 (as_mref r) (as_mref r')
 
 let lemma_free_mm_unused (#a:Type) (#b:Type) (h0:heap) (r:ref a{h0 `contains` r /\ is_mm r}) (r':ref b)
   :Lemma (requires True)
@@ -113,26 +177,26 @@ let lemma_free_mm_unused (#a:Type) (#b:Type) (h0:heap) (r:ref a{h0 `contains` r 
 		     (r' `unused_in` h0      ==> r' `unused_in` h1)      /\
 		     (r' `unused_in` h1      ==> (r' `unused_in` h0 \/ addr_of r' = addr_of r)))))
 	 [SMTPat (r' `unused_in` (free_mm h0 r))]
-  = lemma_free_mm_unused_m h0 r r'
+  = lemma_free_mm_unused_m h0 (as_mref r) (as_mref r')
 
 let lemma_sel_same_addr (#a:Type) (h:heap) (r1:ref a) (r2:ref a)
   :Lemma (requires (h `contains` r1 /\ addr_of r1 = addr_of r2))
          (ensures  (h `contains` r2 /\ sel h r1 == sel h r2))
 	 [SMTPat (sel h r1); SMTPat (sel h r2)]
-  = lemma_sel_same_addr h r1 r2
+  = lemma_sel_same_addr h (as_mref r1) (as_mref r2)
 
 let lemma_sel_upd1 (#a:Type) (h:heap) (r:ref a) (x:a) (r':ref a)
   :Lemma (requires (addr_of r = addr_of r'))
          (ensures  (sel (upd h r x) r' == x))
          [SMTPat (sel (upd h r x) r')]
 
-  = lemma_sel_upd1 h r x r'
+  = lemma_sel_upd1 h (as_mref r) x (as_mref r')
 
 let lemma_sel_upd2 (#a:Type) (#b:Type) (h:heap) (r1:ref a) (r2:ref b) (x:b)
   :Lemma (requires (addr_of r1 <> addr_of r2))
          (ensures  (sel (upd h r2 x) r1 == sel h r1))
 	 [SMTPat (sel (upd h r2 x) r1)]
-  = lemma_sel_upd2 h r1 r2 x
+  = lemma_sel_upd2 h (as_mref r1) (as_mref r2) x
 
 let lemma_ref_injectivity
   :(u:unit{forall (a:Type) (b:Type) (r1:ref a) (r2:ref b). a =!= b ==> ~ (eq3 r1 r2)})
@@ -153,20 +217,20 @@ let lemma_in_dom_emp (#a:Type) (r:ref a)
   :Lemma (requires True)
          (ensures  (r `unused_in` emp))
 	 [SMTPat (r `unused_in` emp)]
-  = lemma_in_dom_emp r
+  = lemma_in_dom_emp (as_mref r)
 
 let lemma_upd_contains (#a:Type) (h:heap) (r:ref a) (x:a)
   :Lemma (requires True)
          (ensures  ((upd h r x) `contains` r))
 	 [SMTPat ((upd h r x) `contains` r)]
-  = lemma_upd_contains h r x
+  = lemma_upd_contains h (as_mref r) x
 
 let lemma_well_typed_upd_contains (#a:Type) (#b:Type) (h:heap) (r:ref a) (x:a) (r':ref b)
   :Lemma (requires (h `contains` r))
          (ensures  (let h1 = upd h r x in
 	            h1 `contains` r' <==> h `contains` r'))
 	 [SMTPat ((upd h r x) `contains` r')]
-  = lemma_well_typed_upd_contains h r x r'
+  = lemma_well_typed_upd_contains h (as_mref r) x (as_mref r')
 
 let lemma_unused_upd_contains (#a:Type) (#b:Type) (h:heap) (r:ref a) (x:a) (r':ref b)
   :Lemma (requires (r `unused_in` h))
@@ -174,13 +238,13 @@ let lemma_unused_upd_contains (#a:Type) (#b:Type) (h:heap) (r:ref a) (x:a) (r':r
 	            (h `contains` r'  ==> h1 `contains` r') /\
 		    (h1 `contains` r' ==> (h `contains` r' \/ addr_of r' = addr_of r))))
 	 [SMTPat ((upd h r x) `contains` r')]
-  = lemma_unused_upd_contains h r x r'
+  = lemma_unused_upd_contains h (as_mref r) x (as_mref r')
 
 let lemma_upd_contains_different_addr (#a:Type) (#b:Type) (h:heap) (r:ref a) (x:a) (r':ref b)
   :Lemma (requires (h `contains` r' /\ addr_of r <> addr_of r'))
          (ensures  ((upd h r x) `contains` r'))
 	 [SMTPat ((upd h r x) `contains` r')]
-  = lemma_upd_contains_different_addr h r x r'
+  = lemma_upd_contains_different_addr h (as_mref r) x (as_mref r')
 
 
 (* let upd_contains (#a:Type) (#b:Type) (h:heap) (r:ref a) (x:a) (r':ref b) *)
@@ -200,19 +264,19 @@ let lemma_upd_unused (#a:Type) (#b:Type) (h:heap) (r:ref a) (x:a) (r':ref b)
   :Lemma (requires True)
          (ensures  ((addr_of r <> addr_of r' /\ r' `unused_in` h) <==> r' `unused_in` (upd h r x)))
 	 [SMTPat (r' `unused_in` (upd h r x))]
-  = lemma_upd_unused h r x r'
+  = lemma_upd_unused h (as_mref r) x (as_mref r')
 
 let lemma_contains_upd_modifies (#a:Type) (h:heap) (r:ref a) (x:a)
   :Lemma (requires (h `contains` r))
          (ensures  (modifies (Set.singleton (addr_of r)) h (upd h r x)))
          [SMTPat (upd h r x); SMTPat (h `contains` r)]
-  = lemma_contains_upd_modifies h r x
+  = lemma_contains_upd_modifies h (as_mref r) x
 
 let lemma_unused_upd_modifies (#a:Type) (h:heap) (r:ref a) (x:a)
   :Lemma (requires (r `unused_in` h))
          (ensures  (modifies (Set.singleton (addr_of r)) h (upd h r x)))
          [SMTPat (upd h r x); SMTPat (r `unused_in` h)]
-  = lemma_unused_upd_modifies h r x
+  = lemma_unused_upd_modifies h (as_mref r) x
 
 (* let lemma_modifies_trans (h1:heap) (h2:heap) (h3:heap) (s1:set nat) (s2:set nat) *)
 (*   :Lemma (requires (modifies s1 h1 h2 /\ modifies s2 h2 h3)) *)
@@ -231,7 +295,7 @@ let upd_upd_same_ref (#a:Type) (h:heap) (r:ref a) (x:a) (y:a)
   :Lemma (requires True)
          (ensures  (upd (upd h r x) r y == upd h r y))
 	 [SMTPat (upd (upd h r x) r y)]
-  = assert (equal (upd (upd h r x) r y) (upd h r y))
+  = () //assert (equal (upd (upd h r x) r y) (upd h r y))
 
 val op_Hat_Plus_Plus: #a:Type -> r:ref a -> set nat -> GTot (set nat)
 let op_Hat_Plus_Plus #a r s = union (only r) s
@@ -242,3 +306,11 @@ let op_Plus_Plus_Hat #a s r = union s (only r)
 val op_Hat_Plus_Hat: #a:Type -> #b:Type -> ref a -> ref b -> GTot (set nat)
 let op_Hat_Plus_Hat #a #b r1 r2 = union (only r1) (only r2)
 
+
+(* lemmas to pass regressions *)
+
+(*let lemma_fresh_not_contained (#a:Type) (r:ref a) (h0:heap) (h1:heap) 
+  :Lemma (requires (fresh r h0 h1))
+         (ensures  (~(contains h0 r)))
+	 [SMTPat (fresh r h0 h1)]
+  = () //lemma_fresh_not_contained r h0 h1*)
